Cm/Pi/Util.lean
@@ -14,11 +14,13 @@ def quote (e : Expr) : Expr :=
 /-
 There is a distinction between loading dowm from higher binders
 and pushing up from lower binders.
+
+I think these are just inverses of each other.
 -/
-notation "var.read" => (fun (n : ℕ) (e : Expr) => List.foldr Expr.cons e (List.replicate n Expr.const))
+notation "var.read" => (fun (n : ℕ) => List.foldr Expr.cons Expr.id (List.replicate n Expr.const))
 -- returning a variable. this corresponds to (:: both (:: (quote const) id))
-notation "var.store" => (fun (n : ℕ) (e : Expr) => List.foldr (fun _e acc  => (:: both (:: (:: const const) acc)))
-  e (List.replicate n (:: const const)))
+notation "var.store" => (fun (n : ℕ) => List.foldr (fun _e acc  => (:: both (:: (:: const const) acc)))
+  Expr.id (List.replicate n (:: const const)))
 
 def mk_binder (n : ℕ) (e : Expr) :=
   match n with
@@ -29,25 +31,43 @@ def mk_binder (n : ℕ) (e : Expr) :=
 
 notation "λ'" => mk_binder
 
+#eval try_step_n' 100 (:: apply (:: (:: apply
+  (:: (λ' 1 (
+    (λ' 2 (:: (var.read 0) (var.read 1)))))
+      (quote (symbol "var 0"))))
+      (quote (symbol "var 1"))))
+
 example : try_step_n' 10 (:: apply (:: (:: apply
   (:: (λ' 1 (
-    (λ' 2 (:: (var.read 1 id) (var.read 1 id)))))
+    (λ' 2 (:: (var.read 1) (var.read 1)))))
       (quote (symbol "var 0"))))
       (quote (symbol "var 1")))) =
     (.ok (:: (:: const (symbol "var 1")) (:: const (symbol "var 1")))) := rfl
 
 example : try_step_n' 10 (:: apply (:: (:: apply
   (:: (λ' 1
-    (λ' 2 (:: (var.read 1 id) (var.read 1 id))))
+    (λ' 2 (:: (var.read 1) (var.read 1))))
       (quote (symbol "var 0"))))
       (quote (symbol "var 1")))) =
     (.ok (:: (:: const (symbol "var 1")) (:: const (symbol "var 1")))) := rfl
 
 example : try_step_n' 10 (:: apply (:: (:: apply
   (:: (:: both (:: (quote both)
-    (:: both (:: (var.store 1 id) (var.store 1 id)))))
+    (:: both (:: (var.store 1) (var.store 1)))))
   (quote (symbol "var 0")))) (quote (symbol "var 1")))) =
     (.ok (:: (:: const (symbol "var 0")) (:: const (symbol "var 0")))) := rfl
+
+example : try_step_n' 1 (:: apply (:: (λ' 0 (var.read 0)) (quote (symbol "var 0")))) = (.ok (:: const (symbol "var 0"))) := rfl
+
+/-
+(:: apply (:: (:: apply (:: (:: apply (:: fun.comp f)) g)) x))
+= (:: apply (:: f (:: apply (:: g x))))
+-/
+def func.comp : Expr := (λ' 1 (λ' 2 (λ' 3 (:: (var.read 2) (:: (var.read 1) (var.read 0))))))
+
+#eval try_step_n 200 (:: apply (:: (:: apply (:: (:: apply (:: func.comp (quote id))) (quote id))) (quote (symbol "hi"))))
+
+--infixr:65 "∘''" => 
 
 /-
 Composition of functions:
